### 1.3 高斯分布
$$
\rho(x) = A\mathrm{e}^{-\lambda(x-a)^{2}} \tag{1.1}
$$
$(a)$
由
$$
\int_{0}^{\infty} \mathrm{e}^{-\lambda x^{2}} \, dx  = \frac{1}{2}\sqrt{ \frac{\pi}{\lambda} } \tag{1.2}
$$
$$
\int_{-\infty}^{+\infty} \rho(x) \, dx = 1 \tag{1.3}
$$
可知
$$
A = \sqrt{ \frac{\lambda}{\pi} }
$$

$(b)$
$$
\langle x \rangle = \int_{-\infty}^{+\infty} x\rho(x) \, dx = a
$$
$$
\langle x^{2} \rangle = \int_{-\infty}^{+\infty} x^{2}\rho(x) \, dx = a^{2}+\frac{1}{2\lambda}
$$
$$
\sigma = \sqrt{ \frac{1}{2\lambda} }
$$
$(c)$

<script src="https://gist.github.com/JianingZhangnan/7bf0c170e183c94e0f39e2bb65f0b7d7.js"></script>

### 1.7
计算$\frac{\mathrm{d}\langle p \rangle}{\mathrm{d}t}$
$$
\langle p \rangle = -\mathrm{i}\hbar \int \Psi^{*}\frac{ \partial \Psi }{ \partial x }  \, dx 
$$
薛定谔方程
$$
\mathrm{i}\hbar \frac{ \partial \Psi  }{ \partial t } =-\frac{\hbar^{2}}{2m} \frac{ \partial^{2} \Psi }{ \partial x^{2} } +V\Psi  
$$
$$
\frac{ \partial \Psi }{ \partial t } = \frac{\mathrm{i}\hbar}{2m} \frac{ \partial^{2} \Psi }{ \partial x^{2} }-\frac{\mathrm{i}V}{\hbar} \Psi
$$
$$
\frac{ \partial^{2} \Psi }{\partial t \partial x } = \frac{\mathrm{i}\hbar}{2m}\frac{ \partial^{3} \Psi }{ \partial x^{3} } - \frac{\mathrm{i}V}{\hbar}\frac{ \partial \Psi }{ \partial x }  -\frac{\Psi \mathrm{i}}{\hbar}\frac{ \partial V }{ \partial x } 
$$
$$
\frac{ \partial \Psi^{*} }{ \partial t } = -\frac{\mathrm{i}\hbar}{2m}\frac{ \partial^{2} \Psi^{*} }{ \partial x^{2} } + \frac{\mathrm{i}V}{\hbar}\Psi^{*}
$$
$$
\begin{align}
\frac{\mathrm{d}\langle p \rangle }{\mathrm{d}t} & = -\mathrm{i}\hbar \int \frac{ \partial \Psi^{*} }{ \partial t } \frac{ \partial \Psi }{ \partial x } +\Psi^{*}\frac{ \partial^{2}  \Psi }{\partial t \partial x }  \, dx  \\
 &  =- i\hbar \int \left( \left( -\frac{\mathrm{i}\hbar}{2m}\frac{ \partial^{2} \Psi^{*} }{ \partial x^{2} } + \frac{\mathrm{i}V}{\hbar}\Psi^{*} \right)\frac{ \partial \Psi }{ \partial x }+\Psi^{*}\left( \frac{\mathrm{i}\hbar}{2m}\frac{ \partial^{3} \Psi }{ \partial x^{3} } - \frac{\mathrm{i}V}{\hbar}\frac{ \partial \Psi }{ \partial x } -\mathrm{\frac{i\Psi}{\hbar}}\frac{ \partial V }{ \partial x }  \right) \right)  \, dx  \\
 & =-\mathrm{i}\hbar \cdot   \int \frac{\mathrm{i}\hbar}{2m}\left( -\frac{ \partial^{2} \Psi^{*} }{ \partial x^{2} } \frac{ \partial \Psi }{ \partial x } +\Psi^{*} \frac{ \partial^{3} \Psi }{ \partial x^{3} }  \right)-\Psi^{*}\mathrm{\frac{i}{\hbar}}\frac{ \partial V }{ \partial x } \Psi \, dx  \\
 & = -\int \Psi^{*}\frac{ \partial V }{ \partial x } \Psi \, dx + \frac{\hbar^{2}}{2m}\int \left( -\frac{ \partial^{2} \Psi^{*} }{ \partial x^{2} } \frac{ \partial \Psi }{ \partial x } +\Psi^{*}\frac{ \partial^{3} \Psi }{ \partial x^{3} }  \right) \, dx  \\
 & = -\left\langle  \frac{ \partial V }{ \partial x }   \right\rangle +\frac{\hbar^{2}}{2m}\int \left( -\frac{ \partial^{2} \Psi^{*} }{ \partial x^{2} } \frac{ \partial \Psi }{ \partial x } +\Psi^{*}\frac{ \partial^{3} \Psi }{ \partial x^{3} }  \right) \, dx
\end{align} 
$$

而
$$
\begin{align}
\int \frac{ \partial^{2} \Psi^{*} }{ \partial x^{2} } \frac{ \partial \Psi }{ \partial x }  \, dx  & = \frac{ \partial \Psi^{*} }{ \partial x } \frac{ \partial \Psi }{ \partial x } \bigg{|}^{+\infty }_{-\infty}- \int \frac{ \partial \Psi^{*} }{ \partial x } \frac{ \partial^{2} \Psi }{ \partial x^{2} }  \, dx  \\
& = -\left( \Psi^{*}\frac{ \partial^{2} \Psi }{ \partial x^{2} }  \right)\bigg{|}^{+\infty}_{-\infty }+\int \Psi^{*}\frac{ \partial^{3} \Psi }{ \partial x^{3} }  \, dx  \\
 & =\int \Psi^{*}\frac{ \partial^{3} \Psi }{ \partial x^{3} }  \, dx 
\end{align}
$$

故
$$
\frac{\hbar^{2}}{2m}\int \left( -\frac{ \partial^{2} \Psi^{*} }{ \partial x^{2} } \frac{ \partial \Psi }{ \partial x } +\Psi^{*}\frac{ \partial^{3} \Psi }{ \partial x^{3} }  \right) \, dx=0
$$
$$
\frac{\mathrm{d}\langle p \rangle }{\mathrm{d}t}=\left\langle  -\frac{ \partial V }{ \partial x }   \right\rangle \tag{1.4}
$$
